mm0-lean/x86/matching.lean
@@ -1,0 +1,465 @@
+import x86.x86 data.set.lattice data.list.basic data.pfun
+
+namespace x86
+
+inductive flag_place | CFP | ZFP | SFP | OFP
+
+def flag_place.read (f : flags) : flag_place → bool
+| flag_place.CFP := f.CF
+| flag_place.ZFP := f.ZF
+| flag_place.SFP := f.SF
+| flag_place.OFP := f.OF
+
+def flag_place.write (f : flags) (b : bool) : flag_place → flags
+| flag_place.CFP := {CF := b, ..f}
+| flag_place.ZFP := {ZF := b, ..f}
+| flag_place.SFP := {SF := b, ..f}
+| flag_place.OFP := {OF := b, ..f}
+
+inductive place
+| flag : flag_place → place
+| reg : regnum → place
+| rip : place
+| mem : qword → place
+
+inductive place.read (k : config) : place → ∀ {n}, bitvec n → Prop
+| flag {f} : place.read (place.flag f) (bitvec.singleton (f.read k.flags))
+| reg {r} : place.read (place.reg r) (k.regs r)
+| rip : place.read place.rip k.rip
+| mem {a b} : k.mem.read1 perm.R a b → place.read (place.mem a) b
+
+inductive place.write (k : config) : place → ∀ {n}, bitvec n → config → Prop
+| flag {f b} : place.write (place.flag f) (bitvec.singleton b) {flags := f.write k.flags b, ..k}
+| reg {r n q} : place.write (place.reg r) q (k.write_reg r n q)
+| rip {q} : place.write place.rip q {rip := q, ..k}
+| mem {a b m'} : k.mem.write1 a b m' → place.write (place.mem a) b {mem := m', ..k}
+
+def place.stable (k k' : config) : place → Prop
+| (place.flag f) := f.read k.flags = f.read k'.flags
+| (place.reg r) := k.regs r = k'.regs r
+| place.rip := k.rip = k'.rip
+| (place.mem a) :=
+  roption.mk (k.mem.valid a) (λ h, (k.mem.mem a h, k.mem.perm a h)) =
+  roption.mk (k'.mem.valid a) (λ h, (k'.mem.mem a h, k'.mem.perm a h))
+
+def stability (k k' : config) : set place := {p | place.stable k k' p}
+
+def split (H h₁ h₂ : set place) : Prop :=
+H = h₁ ∪ h₂ ∧ disjoint h₁ h₂
+
+def sProp := config → Prop
+
+def sProp.reserve (S : set place) : sProp :=
+λ k, ∀ p ∈ S, ∃ n v, @place.read k p n v
+
+def mProp := config → config → Prop
+
+def mProp.exterior (P : mProp) : set place :=
+{p | ∀ k k', P k k' → place.stable k k' p}
+
+def initial (P : sProp) : mProp := λ k _, P k
+def final (P : sProp) : mProp := λ _ k, P k
+
+def mProp.apply (Q : mProp) (P : sProp) : sProp :=
+λ k', ∃ k, P k ∧ Q k k'
+
+def mProp.comp (P Q : mProp) : mProp :=
+λ k k₂, ∃ k₁, P k k₁ ∧ Q k₁ k₂
+
+def slift (p : Prop) : sProp := λ _, p
+def mlift (p : Prop) : mProp := λ _ _, p
+
+def sProp.and (P Q : sProp) : sProp := λ k, P k ∧ Q k
+def mProp.and (P Q : mProp) : mProp := λ k k', P k k' ∧ Q k k'
+def sProp.or (P Q : sProp) : sProp := λ k, P k ∨ Q k
+def mProp.or (P Q : mProp) : mProp := λ k k', P k k' ∨ Q k k'
+instance lattice.has_inf.sProp : lattice.has_inf sProp := ⟨sProp.and⟩
+instance lattice.has_inf.mProp : lattice.has_inf mProp := ⟨mProp.and⟩
+instance lattice.has_sup.sProp : lattice.has_sup sProp := ⟨sProp.or⟩
+instance lattice.has_sup.mProp : lattice.has_sup mProp := ⟨mProp.or⟩
+
+def sProp.with (p : sProp) (q : Prop) : sProp := p ⊓ slift q
+def mProp.with (p : mProp) (q : Prop) : mProp := p ⊓ mlift q
+
+def sProp.ex {α} (p : α → sProp) : sProp := λ k, ∃ a, p a k
+def mProp.ex {α} (p : α → mProp) : mProp := λ k k', ∃ a, p a k k'
+
+def sProp.al {α} (p : α → sProp) : sProp := λ k, ∀ a, p a k
+def mProp.al {α} (p : α → mProp) : mProp := λ k k', ∀ a, p a k k'
+
+def sProp.sn (p : place) {n} (v : bitvec n) : sProp :=
+λ k, p.read k v
+def mProp.write (p : place) {n} (v' : bitvec n) : mProp :=
+λ k k', p.write k v' k'
+def mProp.sn (p : place) {n} (v v' : bitvec n) : mProp :=
+initial (sProp.sn p v) ⊓ mProp.write p v'
+def mProp.clob (p : place) {n} (v : bitvec n) : mProp :=
+mProp.ex $ λ v', mProp.sn p v v'
+
+def sProp.flags (f : flags) : sProp :=
+sProp.al $ λ p : flag_place,
+sProp.sn (place.flag p) (bitvec.singleton $ p.read f)
+
+inductive block
+| reg : regnum → wsize → block
+| mem : qword → qword → block
+| const : list byte → block
+
+def block.size : block → qword
+| (block.reg _ sz) := (sz.to_nat / 8 : ℕ)
+| (block.mem _ sz) := sz
+| (block.const l) := l.length
+
+inductive block.places : block → set place
+| reg {r sz} : block.places (block.reg r sz) (place.reg r)
+| mem {a b sz : qword} :
+  (bitvec.sub b a).to_nat ≤ sz.to_nat →
+  block.places (block.mem a sz) (place.mem b)
+
+def block.disj (b1 b2 : block) := disjoint b1.places b2.places
+
+def sProp.mem_block (p : perm) (a : qword) (v : list byte) : sProp :=
+λ k, k.mem.read' p a v
+
+def block.read : block → list byte → sProp
+| (block.reg r sz) v :=
+  (sProp.reserve (block.reg r sz).places).and $ λ k,
+    read_full_imm sz (k.regs r) v
+| (block.mem a sz) v :=
+  (sProp.reserve (block.mem a sz).places).and $ λ k,
+    k.mem.read a v ∧ v.length = sz.to_nat
+| (block.const l) v := slift $ v = l
+
+def block.writable : block → sProp
+| (block.reg r sz) := sProp.reserve (block.reg r sz).places
+| (block.mem a sz) :=
+  (sProp.reserve (block.mem a sz).places).and $ λ k,
+    ∃ v, k.mem.read' perm.W a v ∧ v.length = sz.to_nat
+| (block.const _) := slift false
+
+def block.write : block → list byte → mProp
+| (block.reg r sz) l k k' := ∃ v,
+  @bits_to_byte (sz.to_nat * 8) sz.to_nat v l ∧
+  mProp.write (place.reg r) v k k'
+| (block.mem a sz) l k k' :=
+  ∃ m', k.mem.write a l m' ∧ k' = {mem := m', ..k}
+| (block.const _) _ _ _ := false
+
+theorem block.read.size : ∀ {b v k},
+  block.read b v k → v.length = b.size.to_nat := sorry
+
+theorem block.write.size : ∀ {b v k k'},
+  block.write b v k k' → v.length = b.size.to_nat := sorry
+
+theorem block.read_write : ∀ {b v k k'},
+  block.write b v k k' → block.read b v k' := sorry
+
+theorem block.read.stable {l v k k'}
+  (h₁ : block.read l v k) (ss : places l ⊆ stability k k') :
+  block.read l v k' := sorry
+
+def locals_ctx (n : ℕ) := {Γ : list (ℕ × block) //
+  Γ.pairwise (λ i j, i.1 ≠ j.1 ∧ i.2.disj j.2) ∧
+  ∀ i : ℕ × block, i ∈ Γ → i.1 < n}
+
+instance {n} : has_mem (ℕ × block) (locals_ctx n) := ⟨λ a Γ, a ∈ Γ.1⟩
+
+def locals_ctx.cons {n} (Γ : locals_ctx n) (b : block)
+  (h : ∀ i : ℕ × block, i ∈ Γ → b.disj i.2) : locals_ctx (n+1) :=
+⟨(n, b) :: Γ.1,
+  list.pairwise_cons.2 ⟨λ i h', ⟨ne_of_gt $ Γ.2.2 _ h', h _ h'⟩, Γ.2.1⟩,
+  by rintro i (rfl|h'); [
+    apply nat.lt_succ_self,
+    exact nat.lt_succ_of_lt (Γ.2.2 _ h')]⟩
+
+def locals_ctx.shrink {m n} (Γ : locals_ctx m) : locals_ctx n :=
+⟨Γ.1.filter (λ i, i.1 < n),
+  list.pairwise_of_sublist (list.filter_sublist _) Γ.2.1,
+  λ i h, (list.mem_filter.1 h).2⟩
+
+def labels_ctx := qword × list qword
+
+def labels_ctx.cons (q : qword) (L : labels_ctx) : labels_ctx :=
+⟨L.1, q :: L.2⟩
+
+inductive hoare_p (Q : kcfg → Prop) : kcfg → Prop
+| zero {{k}} : Q k → hoare_p k
+| step {{k}} : (∃ k', kcfg.step k k') →
+  (∀ k', k.step k' → hoare_p k') → hoare_p k
+| exit (k : kcfg) (ret) :
+  k.k.exit ret → (ret = 0 → Q k) → hoare_p k
+
+def hoare (P Q : kcfg → Prop) :=
+∀ {{k}}, P k → hoare_p Q k
+
+def sHoareIO (P : sProp) (Q : list byte → list byte → sProp) :=
+∀ {{i o}}, hoare (λ k, P k.k ∧ k.input = i ∧ k.output = o)
+  (λ k, ∃ i' o', i = i' ++ k.input ∧ o = k.output ++ o' ∧
+    (Q i' o') k.k)
+def mHoareIO (P : sProp) (Q : list byte → list byte → mProp) :=
+sHoareIO P (λ i o, (Q i o).apply P)
+
+def noIO (Q : mProp) (i o : list byte) : mProp := Q.with (i = [] ∧ o = [])
+def mHoare (P : sProp) (Q : mProp) := mHoareIO P (noIO Q)
+
+inductive exit_kind
+| straight
+| label (n : ℕ)
+
+def exit_kind.result (L : labels_ctx) (pos : qword) : exit_kind → mProp
+| exit_kind.straight := mProp.write place.rip pos
+| (exit_kind.label n) := mProp.ex $ λ h, mProp.write place.rip (L.2.nth_le n h)
+
+def stmt (n) : Type :=
+labels_ctx → locals_ctx n →
+∀ rip : qword, list byte → Prop
+
+def stmt.hoareIO (P : sProp) {n} (C : stmt n)
+  (Q : exit_kind → list byte → list byte → mProp) : Prop :=
+∀ L Γ rip l, C L Γ rip l →
+  mHoareIO (P ⊓ sProp.sn place.rip rip ⊓ sProp.mem_block (perm.R + perm.X) rip l)
+    (λ i o,
+      mProp.write place.rip L.1 ⊔
+      mProp.ex (λ e, Q e i o ⊓ e.result L (rip + l.length)))
+
+def stmt.hoare (P : sProp) {n} (C : stmt n) (Q : exit_kind → mProp) : Prop :=
+stmt.hoareIO P C (λ e, noIO (Q e))
+
+def hstmt {n} (P : sProp) (Q : mProp) : stmt n :=
+λ L Γ rip v,
+  mHoare (sProp.sn place.rip rip ⊓ sProp.mem_block (perm.R + perm.X) rip v)
+    (Q ⊓ mProp.write place.rip (rip + v.length))
+
+def stmt.all {α n} (s : α → stmt n) : stmt n :=
+λ L Γ rip v, ∀ a, s a L Γ rip v
+
+def stmt.ex {α n} (s : α → stmt n) : stmt n :=
+λ L Γ rip v, ∃ a, s a L Γ rip v
+
+def stmt.with {n} (p : Prop) (s : stmt n) : stmt n :=
+stmt.ex $ λ h : p, s
+
+def stmt.or {n} (s₁ s₂ : stmt n) : stmt n :=
+λ L Γ rip v, s₁ L Γ rip v ∨ s₂ L Γ rip v
+
+def stmt.lift {m n} (s : stmt n) : stmt m := λ L Γ, s L Γ.shrink
+
+def expr (n) := block → stmt n
+
+def expr.hoareIO (P : sProp) {n} (E : expr n)
+  (Q : block → list byte → list byte → mProp) : Prop :=
+∀ b, (E b).hoareIO P $
+  λ e i o, exit_kind.cases_on e (Q b i o) (λ n, mlift false)
+
+def expr.hoare (P : sProp) {n} (E : expr n) (Q : block → mProp) : Prop :=
+expr.hoareIO P E (λ ret, noIO (Q ret))
+
+def expr.lift {m n} (e : expr n) : expr m := λ b, stmt.lift (e b)
+
+class value (α : Type*) :=
+(size : ℕ)
+(eval : α → list byte → Prop)
+(eval_eq : ∀ {{a l}}, eval a l → l.length = size)
+
+def value.evalB {α} [value α] (x : α) (b : block) : sProp :=
+λ k, ∃ l, block.read b l k ∧ value.eval x l
+
+def value.read_sized {α} [value α] (a : qword) (x : α) (b : block) : sProp :=
+value.evalB x b ⊓ slift (b = block.mem a (value.size α))
+
+class type (α : Type*) :=
+(size : ℕ)
+(read : α → block → set place → sProp)
+(write : α → block → mProp)
+(read_eq : ∀ {{a l s k}}, read a l s k → l.size.to_nat = size)
+(write_eq : ∀ {{a l k k'}}, write a l k k' → l.size.to_nat = size)
+(read_write : ∀ {{a l k k'}}, write a l k k' → ∃ s, read a l s k')
+(read_stable : ∀ {{a l s k k'}},
+  read a l s k → s ⊆ stability k k' → read a l s k')
+
+instance (α) [value α] : type α :=
+⟨value.size α,
+  λ a b s, sProp.ex $ λ v,
+    block.read b v ⊓ slift (value.eval a v ∧ s = b.places),
+  λ a b, mProp.ex $ λ v,
+    block.write b v ⊓ mlift (value.eval a v),
+  λ a b s k ⟨v, h₁, h₂, _⟩, by rw [← h₁.size, @value.eval_eq α _ a v h₂],
+  λ a b k k' ⟨v, h₁, h₂⟩, by rw [← h₁.size, @value.eval_eq α _ a v h₂],
+  λ a v k k' ⟨s, h₁, h₂⟩, ⟨_, _, block.read_write h₁, h₂, rfl⟩,
+  λ a l s k k' ⟨v, h₁, h₂, e⟩ ss, ⟨v, h₁.stable (e ▸ ss), h₂, e⟩⟩
+
+def expr.hoareT (P : sProp) {n} (E : expr n) {α} [type α] (Q : α → set place → mProp) : Prop :=
+expr.hoare P E $ λ v,
+mProp.ex $ λ a, mProp.ex $ λ s, Q a s ⊓ final (type.read a v s)
+
+theorem bits_to_byte_length {n m w v} : @bits_to_byte n m w v → v.length = m :=
+by rintro ⟨bs⟩; exact bs.2
+
+def bits.value {n} (m : ℕ) : value (bitvec n) :=
+⟨m, bits_to_byte m, λ a v h, bits_to_byte_length h⟩
+
+instance unit.value : value unit :=
+⟨0, λ _ v, v = [], by rintro _ _ ⟨⟩; refl⟩
+
+instance byte.value : value byte :=
+⟨1, λ b v, v = [b], by rintro _ _ ⟨⟩; refl⟩
+
+instance word.value : value word := bits.value 4
+instance qword.value : value qword := bits.value 8
+
+class box (α) [type α] := (deref : α)
+
+instance box.type (α) [type α] : type (box α) :=
+⟨8, λ x b s k, ∃ a l s',
+    block.read b l k ∧
+    qword.to_list_byte a l ∧
+    type.read x.deref (block.mem a (type.size α)) s' k ∧
+    s = b.places ∪ s',
+  λ x b k k', ∃ a l s',
+    block.write b l k k' ∧
+    qword.to_list_byte a l ∧
+    type.read x.deref (block.mem a (type.size α)) s' k',
+  λ x b s k ⟨a, l, s', h₁, h₂, _⟩,
+    by rw [← h₁.size, bits_to_byte_length h₂],
+  λ x b k k' ⟨a, l, s', h₁, h₂, _⟩,
+    by rw [← h₁.size, bits_to_byte_length h₂],
+  λ x b k k' ⟨a, l, s', h₁, h₂, h₃⟩,
+    ⟨_, _, _, _, block.read_write h₁, h₂, h₃, rfl⟩,
+  λ x b s k k' ⟨a, l, s', h₁, h₂, h₃, e⟩ ss,
+    let ⟨ss₁, ss₂⟩ := set.union_subset_iff.1 (by rwa e at ss) in
+    ⟨a, l, s', h₁.stable ss₁, h₂, type.read_stable h₃ ss₂, e⟩⟩
+
+def const {n} (l : list byte) : expr n :=
+λ bl L Γ a v, bl = block.const l ∧ v = []
+
+def var {n} (i : ℕ) : expr n :=
+λ bl L Γ a v, (i, bl) ∈ Γ.1 ∧ v = []
+
+def hexpr {n} (P : sProp) (Q : block → mProp) : expr n :=
+λ ret, hstmt P (Q ret)
+
+def expr.all {α n} (e : α → expr n) : expr n :=
+λ ret, stmt.all $ λ a, e a ret
+
+def expr.ex {α n} (e : α → expr n) : expr n :=
+λ ret, stmt.ex $ λ a, e a ret
+
+def expr.with {n} (p : Prop) (s : expr n) : expr n :=
+expr.ex $ λ h : p, s
+
+def const' {n} (sz : wsize) (i : ℕ) : expr n :=
+expr.ex $ λ q, expr.ex $ λ l,
+expr.with (read_full_imm sz q l ∧ q.to_nat = i) $
+const l
+
+inductive stmt.seq {n} (s₁ : stmt n) (s₂ : stmt n) : stmt n
+| mk {L Γ rip v₁ v₂} :
+  s₁ L Γ rip v₁ →
+  s₂ L Γ (rip + v₁.length) v₂ →
+  stmt.seq L Γ rip (v₁ ++ v₂)
+
+inductive expr.bindS {n} (e₁ : expr n) (s₂ : block → stmt n) : stmt n
+| mk {b L Γ rip v₁ v₂} :
+  e₁ b L Γ rip v₁ →
+  s₂ b L Γ (rip + v₁.length) v₂ →
+  expr.bindS L Γ rip (v₁ ++ v₂)
+
+def expr.bind {n} (e₁ : expr n) (e₂ : block → expr n) : expr n :=
+λ b₂, expr.bindS e₁ $ λ b₁, e₂ b₁ b₂
+
+def block.mov {n} (dst src : block) : stmt n :=
+stmt.with (dst.size = src.size) $
+stmt.all $ λ val, hstmt (block.read src val) (block.write dst val)
+
+def expr.set {n} (e₁ e₂ : expr n) : stmt n :=
+expr.bindS e₁ $ λ dst, expr.bindS e₂ $ λ src, block.mov dst src
+
+inductive label | fail | label (n : ℕ)
+
+inductive label.loc (L : labels_ctx) : label → qword → Prop
+| fail : label.loc label.fail L.1
+| label (n h) : label.loc (label.label n) (L.2.nth_le n h)
+
+def stmt.jump_cc {n} (p : flags → bool) (l : label) : stmt n :=
+λ L Γ rip v, ∀ tgt, l.loc L tgt →
+mHoare (sProp.sn place.rip rip ⊓ sProp.mem_block (perm.R + perm.X) rip v)
+  (λ k k', mProp.write place.rip (cond (p k.flags) tgt (rip + v.length)) k k')
+
+def stmt.jump {n} : label → stmt n := stmt.jump_cc (λ _, tt)
+
+def boolexpr (n) := (flags → bool) × stmt n
+
+def boolexpr.hoare (P : sProp) {n} (E : boolexpr n) (Q : bool → mProp) : Prop :=
+stmt.hoare P E.2
+  (λ e k k', e = exit_kind.straight ∧ Q (E.1 k'.flags) k k')
+
+def boolexpr.not {n} (c : boolexpr n) : boolexpr n :=
+⟨λ f, bnot $ c.1 f, c.2⟩
+
+def boolexpr.jump_if {n} (c : boolexpr n) (l : label) : stmt n :=
+stmt.seq c.2 $ stmt.jump_cc c.1 l
+
+def stmt.nop {n} : stmt n := λ L Γ rip v, v = []
+
+def if_stmt {n} (c : boolexpr n) (s₁ s₂ : stmt n) : stmt n :=
+stmt.seq c.not.2 $ λ L Γ rip v,
+∃ v₁ v₂ v₃, v = v₁ ++ v₂ ++ v₃ ∧
+let q₁ := rip + v₁.length, q₂ := q₁ + v₂.length in
+stmt.jump_cc c.not.1 (label.label 0) (L.cons q₁) Γ rip v₁ ∧
+s₁.seq (stmt.jump (label.label 0)) (L.cons q₂) Γ q₁ v₂ ∧
+s₂.seq (stmt.jump (label.label 0)) (L.cons q₂) Γ q₂ v₃
+
+def loop {n} (s : stmt n) : stmt n :=
+λ L Γ rip, s (L.cons rip) Γ rip
+
+def block_stmt {n} (s : stmt n) : stmt n :=
+λ L Γ rip v, s (L.cons (rip + v.length)) Γ rip v
+
+def while {n} (c : boolexpr n) (s : stmt n) : stmt n :=
+block_stmt $ loop $
+  (c.not.jump_if (label.label 1)).seq $
+  s.seq $
+  stmt.jump (label.label 0)
+
+def decl_block {n} (b : block) (s : stmt (n + 1)) : stmt n :=
+λ L Γ rip v, ∀ h, s L (Γ.cons b h) rip v
+
+def decl {n} (sz : qword) (s : stmt (n + 1)) : stmt n :=
+λ L Γ rip v, ∀ b h, block.size b = sz → s L (Γ.cons b h) rip v
+
+def init_rvo {n} (sz : qword) (e : expr n) (s : stmt (n + 1)) : stmt n :=
+e.bindS $ λ b, stmt.with (b.size = sz) $
+λ L Γ rip v, ∃ h, s L (Γ.cons b h) rip v
+
+def init_assign {n} (sz : qword) (e : expr n) (s : stmt (n + 1)) : stmt n :=
+e.bindS $ λ b, stmt.with (b.size = sz) $
+decl sz $ ((var n).set e.lift).seq s
+
+def init {n} (sz : qword) (e : expr n) (s : stmt (n + 1)) : stmt n :=
+(init_rvo sz e s).or (init_assign sz e s)
+
+def for {n} (sz : qword) (start : expr n)
+  (test : boolexpr (n+1)) (incr body : stmt (n+1)) : stmt n :=
+init sz start $ while test $ body.seq incr
+
+def binop_expr {n α β γ} [type α] [type β]
+  (f : α → β → γ) (mk : γ → list byte → Prop)
+  (e₁ e₂ : expr n) : expr n :=
+e₁.bind $ λ b₁, e₂.bind $ λ b₂,
+sorry
+
+def incr {n} (i) : stmt n :=
+(var i).set $ binop_expr (+) qword.to_list_byte (var i) (const [1])
+
+def bool_binop {n α β} [type α] [type β]
+  (f : α → β → bool) (e₁ e₂ : expr n) : boolexpr n :=
+⟨sorry, e₁.bindS $ λ b₁, e₂.bindS $ λ b₂,
+  sorry⟩
+
+def lt {n} (e₁ e₂ : expr n) : boolexpr n :=
+bool_binop (λ a b : qword, a.to_nat < b.to_nat) e₁ e₂
+
+def for_seq {n} (sz : qword) (max : expr n) (body : stmt (n+1)) : stmt n :=
+for sz (const' wsize.Sz64 0) (lt (const' wsize.Sz64 0) max.lift) (incr n) body
+
+end x86
